in the middle of fixing commute lemmas premises + cleaned up measure decrease lemma and moved clock invariant lemmas to EP+_Trace

txn-data-consistency/EP+_Reduction.thy
@@ -1,7 +1,7 @@
 section \<open>Reductions for EP+\<close>
 
 theory "EP+_Reduction"
-  imports "EP+" "EP+_Trace" Reductions
+  imports "EP+_Commutes"
 begin
 
 datatype movt = Lm | Rm | Out
@@ -28,11 +28,11 @@ definition left_most_Lm_dist_left :: "'v ev list \<Rightarrow> nat" where
   "left_most_Lm_dist_left tr \<equiv> let (j, k) = left_most_adj_pair ev_ects tr in
     (THE i. left_most_Lm tr i j k) - j"
 
-definition measure_R :: "('v ev, ('v, 'm) global_conf_scheme) exec_frag rel" where
-  "measure_R \<equiv> measures [card o inverted_pairs ev_ects o trace_of_efrag, lmp_Lm_dist_left o trace_of_efrag]"
-
 definition measure_R' :: "('v ev, ('v, 'm) global_conf_scheme) exec_frag rel" where
-  "measure_R' \<equiv> measures [card o inverted_pairs ev_ects o trace_of_efrag,
+  "measure_R' \<equiv> measures [card o inverted_pairs ev_ects o trace_of_efrag, lmp_Lm_dist_left o trace_of_efrag]"
+
+definition measure_R :: "('v ev, ('v, 'm) global_conf_scheme) exec_frag rel" where
+  "measure_R \<equiv> measures [card o inverted_pairs ev_ects o trace_of_efrag,
                            card o lmp_left_movers o trace_of_efrag,
                            left_most_Lm_dist_left o trace_of_efrag]" \<comment> \<open>Is this better?\<close>
 
@@ -54,292 +54,6 @@ lemma mover_type_in:
 lemma mover_type_out:
   "\<not>(j \<le> i \<and> i \<le> k) \<Longrightarrow> mover_type tr i j k = Out"
   by (auto simp add: mover_type_def)
-
-lemma cts_lt:
-  "cts' > cts \<Longrightarrow> (cts', Suc cl) > (cts, Suc cl)"
-  by (simp add: less_prod_def)
-
-subsubsection \<open>cl_ord clock invariant\<close>
-lemma cl_clock_monotonic:
-  "state_trans s e s' \<Longrightarrow> cl_clock (cls s' cl) \<ge> cl_clock (cls s cl)"
-  by (induction e) (auto simp add: tps_trans_defs)
-
-lemma last_clk_max_in_cl:
-  assumes
-    \<open>tps: s \<midarrow>\<langle>\<tau>\<rangle>\<rightarrow> s'\<close>
-    \<open>reach tps s\<close>
-    \<open>ev_cl (\<tau> ! i) = Some cl\<close>
-    \<open>i < length \<tau>\<close>
-  shows \<open>ev_clk (\<tau> ! i) \<le> cl_clock (cls s' cl)\<close>
-  using assms
-proof (induction \<tau> s' arbitrary: i rule: trace.induct)
-  case (trace_snoc \<tau> s' e s'')
-  then show ?case
-  proof (cases "i = length \<tau>")
-    case True
-    then show ?thesis using trace_snoc
-      by (induction e) (auto simp add: tps_trans_defs)
-  next
-    case False
-    then show ?thesis using trace_snoc
-      apply (simp add: nth_append)
-      using cl_clock_monotonic le_trans not_less_less_Suc_eq by blast
-  qed
-qed simp
-
-lemma cl_ord_implies_clk_order:
-  assumes
-    \<open>tps: s \<midarrow>\<langle>\<tau>\<rangle>\<rightarrow> s'\<close>
-    \<open>reach tps s\<close>
-    \<open>(\<tau> ! j, \<tau> ! k) \<in> cl_ord\<close>
-    \<open>j < k\<close>
-    \<open>k < length \<tau>\<close>
-  shows \<open>ev_clk (\<tau> ! j) < ev_clk (\<tau> ! k)\<close>
-  using assms
-proof (induction \<tau> s' arbitrary: j k rule: trace.induct)
-  case (trace_snoc \<tau> s' e s'')
-  then show ?case
-  proof (cases "k = length \<tau>")
-    case True
-    then show ?thesis using trace_snoc
-      by (induction e)
-        (auto simp add: tps_trans_defs nth_append cl_ord_def last_clk_max_in_cl le_imp_less_Suc,
-          ((meson last_clk_max_in_cl le_imp_less_Suc le_trans max.coboundedI1)+)?)
-  next
-    case False
-    then show ?thesis using trace_snoc by (simp add: nth_append)
-  qed
-qed simp
-
-
-subsubsection \<open>svr_ord clock invariant\<close>
-lemma svr_clock_monotonic:
-  "state_trans s e s' \<Longrightarrow> svr_clock (svrs s' svr) \<ge> svr_clock (svrs s svr)"
-  by (induction e) (auto simp add: tps_trans_defs)
-
-lemma last_clk_max_in_svr:
-  assumes
-    \<open>tps: s \<midarrow>\<langle>\<tau>\<rangle>\<rightarrow> s'\<close>
-    \<open>reach tps s\<close>
-    \<open>ev_key (\<tau> ! i) = Some k\<close>
-    \<open>i < length \<tau>\<close>
-  shows \<open>ev_clk (\<tau> ! i) \<le> svr_clock (svrs s' k)\<close>
-  using assms
-proof (induction \<tau> s' arbitrary: i rule: trace.induct)
-  case (trace_snoc \<tau> s' e s'')
-  then show ?case
-  proof (cases "i = length \<tau>")
-    case True
-    then show ?thesis using trace_snoc
-      by (induction e) (auto simp add: tps_trans_defs)
-  next
-    case False
-    then show ?thesis using trace_snoc
-      apply (simp add: nth_append)
-      using svr_clock_monotonic le_trans not_less_less_Suc_eq by blast
-  qed
-qed simp
-
-lemma svr_ord_implies_clk_order:
-  assumes
-    \<open>tps: s \<midarrow>\<langle>\<tau>\<rangle>\<rightarrow> s'\<close>
-    \<open>reach tps s\<close>
-    \<open>(\<tau> ! j, \<tau> ! k) \<in> svr_ord\<close>
-    \<open>j < k\<close>
-    \<open>k < length \<tau>\<close>
-  shows \<open>ev_clk (\<tau> ! j) < ev_clk (\<tau> ! k)\<close>
-  using assms
-proof (induction \<tau> s' arbitrary: j k rule: trace.induct)
-  case (trace_snoc \<tau> s' e s'')
-  then show ?case
-  proof (cases "k = length \<tau>")
-    case True
-    then show ?thesis using trace_snoc
-      by (induction e)
-        (auto simp add: tps_trans_defs nth_append svr_ord_def last_clk_max_in_svr le_imp_less_Suc,
-          ((meson last_clk_max_in_svr le_imp_less_Suc le_trans max.coboundedI1)+)?)
-  next
-    case False
-    then show ?thesis using trace_snoc by (simp add: nth_append)
-  qed
-qed simp
-
-
-subsubsection \<open>txn_ord clock invariant\<close>
-lemma helper:
-  "x k = Some y \<Longrightarrow> finite (dom x) \<Longrightarrow> f k < Suc (max A (Max {f k |k. k \<in> dom x}))"
-  apply (simp add: Setcompr_eq_image)
-  by (metis Max.coboundedI domI finite_imageI le_imp_less_Suc max.coboundedI1 max.commute not_in_image)
-
-lemma sc_ord_implies_clk_order:
-  assumes
-    \<open>tps: s \<midarrow>\<langle>\<tau>\<rangle>\<rightarrow> s'\<close>
-    \<open>reach tps s\<close>
-    \<open>(\<tau> ! j, \<tau> ! k) \<in> txn_ord\<close>
-    \<open>j < k\<close>
-    \<open>k < length \<tau>\<close>
-  shows \<open>ev_clk (\<tau> ! j) < ev_clk (\<tau> ! k)\<close>
-  using assms
-proof (induction \<tau> s' arbitrary: j k rule: trace.induct)
-  case (trace_snoc \<tau> s' e s'')
-  then show ?case
-  proof (cases "k = length \<tau>")
-    case True
-    then show ?thesis using trace_snoc
-    proof (induction e)
-      case (Read x1 x2 x3 x4 x5 x6 x7)
-      then show ?case 
-      proof (cases "\<tau> ! j")
-        case (RegR x71 x72 x73 x74 x75 x76 x77)
-        then show ?thesis using Read by (simp add: nth_append txn_ord_def tps_trans_defs)
-      qed (simp_all add: nth_append txn_ord_def)
-    next
-      case (WCommit x1 x2 x3 x4 x5 x6 x7)
-      then show ?case 
-      proof (cases "\<tau> ! j")
-        case (PrepW x81 x82 x83 x84 x85)
-        then show ?thesis using WCommit
-          apply (auto simp add: nth_append txn_ord_def tps_trans_defs)
-          using Finite_Dom_Kv_map_def[of s' x1]
-            helper[of x2 x81 _ "\<lambda>k. get_ts (svr_state (svrs s' k) (get_wtxn s' x1))"] 
-          apply simp
-          by (smt not_None_eq option.inject reach_finite_dom_kv_map reach_trace_extend)
-      qed (simp_all add: nth_append txn_ord_def)
-    next
-      case (WDone x1 x2 x3 x4 x5)
-      then show ?case 
-      proof (cases "\<tau> ! j")
-        case (CommitW x91 x92 x93 x94 x95 x96 x97)
-        then show ?thesis using WDone
-          apply (cases "x2 x91", auto simp add: nth_append txn_ord_def tps_trans_defs)
-          using Finite_Dom_Kv_map_def[of s' x1]
-            helper[of x2 x91 _ "\<lambda>k. get_sclk (svr_state (svrs s' k) (get_wtxn s' x1))"] 
-          apply simp
-          by (smt (verit) reach_finite_dom_kv_map reach_trace_extend)
-         qed (simp_all add: nth_append txn_ord_def)
-    next
-      case (RegR x1 x2 x3 x4 x5 x6 x7)
-      then show ?case 
-      proof (cases "\<tau> ! j")
-        case (RInvoke x11 x12 x13 x14)
-        then show ?thesis using RegR by (auto simp add: nth_append txn_ord_def tps_trans_defs)
-      qed (simp_all add: nth_append txn_ord_def)
-    next
-      case (PrepW x1 x2 x3 x4 x5)
-      then show ?case 
-      proof (cases "\<tau> ! j")
-        case (WInvoke x41 x42 x43 x44)
-        then show ?thesis using PrepW by (auto simp add: nth_append txn_ord_def tps_trans_defs)
-      qed (simp_all add: nth_append txn_ord_def)
-    next
-      case (CommitW x1 x2 x3 x4 x5 x6 x7)
-      then show ?case 
-      proof (cases "\<tau> ! j")
-        case (WCommit x51 x52 x53 x54 x55 x56 x57)
-        then show ?thesis using CommitW by (auto simp add: nth_append txn_ord_def tps_trans_defs)
-      qed (simp_all add: nth_append txn_ord_def)
-    qed (auto simp add: txn_ord_def)
-  next
-    case False
-    then show ?thesis using trace_snoc by (simp add: nth_append)
-  qed
-qed simp
-
-
-subsubsection \<open>causal_dep clock invariant\<close>
-lemma causal_dep0_implies_clk_order:
-  assumes
-    \<open>tps: s \<midarrow>\<langle>\<tau>\<rangle>\<rightarrow> s'\<close>
-    \<open>reach tps s\<close>
-    \<open>EVI \<tau> j \<lesssim>\<^sup>0 EVI \<tau> k\<close>
-    \<open>k < length \<tau>\<close>
-  shows \<open>ev_clk (\<tau> ! j) < ev_clk (\<tau> ! k)\<close>
-  using assms
-proof (induction \<tau> s' arbitrary: j k rule: trace.induct)
-  case (trace_snoc \<tau> s' e s'')
-  then show ?case
-  proof (cases "k = length \<tau>")
-    case True
-    then show ?thesis using trace_snoc
-        causal_dep0_nth_append[of \<tau>]
-        causal_dep0_ind_lt[of "EVI (\<tau> @ [e]) j" "EVI (\<tau> @ [e]) k"]
-      apply (auto simp add: causal_dep0_def)
-      subgoal by (metis (mono_tags, lifting) cl_ord_implies_clk_order nth_append_length
-          trace.trace_snoc trace_snoc.hyps(2) trace_snoc.prems(3)) \<comment> \<open>cl_ord\<close>
-      subgoal by (metis (mono_tags, lifting) svr_ord_implies_clk_order nth_append_length
-          trace.trace_snoc trace_snoc.hyps(2) trace_snoc.prems(3)) \<comment> \<open>svr_ord\<close>
-      subgoal by (metis (no_types, lifting) sc_ord_implies_clk_order nth_append_length
-            trace.trace_snoc trace_snoc.hyps(2) trace_snoc.prems(3)) \<comment> \<open>txn_ord\<close>
-      done
-  next
-    case False
-    then show ?thesis using trace_snoc
-        causal_dep0_nth_append[of \<tau>]
-        causal_dep0_ind_lt[of "EVI (\<tau> @ [e]) j" "EVI (\<tau> @ [e]) k"]
-      by (simp add: nth_append)
-    qed
-qed simp
-
-
-lemma causal_dep_implies_clk_order:
-  assumes
-    \<open>tps: s \<midarrow>\<langle>\<tau>\<rangle>\<rightarrow> s'\<close>
-    \<open>reach tps s\<close>
-    \<open>EVI \<tau> j < EVI \<tau> k\<close>
-    \<open>k < length \<tau>\<close>
-  shows \<open>ev_clk (\<tau> ! j) < ev_clk (\<tau> ! k)\<close>
-  using assms(3-)
-  apply (simp add: less_ev_i_def)
-  apply (induction "EVI \<tau> j" "EVI \<tau> k" arbitrary: k rule: trancl.induct)
-  subgoal using assms(1,2) causal_dep0_implies_clk_order by blast
-  subgoal for b k apply (cases b)
-    using assms(1,2) causal_dep0_tr_eq[of b "EVI \<tau> k"]
-      causal_dep0_ind_lt[of b "EVI \<tau> k"] apply auto
-    by (smt (verit, best) add_diff_inverse_nat causal_dep0_implies_clk_order less_SucI
-        not_less_eq trans_less_add1)
-  done
-
-
-lemma WCommit_clk_Suc_cts:
-  assumes
-    \<open>tps: s \<midarrow>\<langle>\<tau>\<rangle>\<rightarrow> s'\<close>
-    \<open>reach tps s\<close>
-    \<open>i < length \<tau>\<close>
-    \<open>\<tau> ! i = WCommit cl kv_map cts sn u'' clk mmap\<close>
-  shows \<open>clk = Suc cts\<close>
-  using assms
-proof (induction \<tau> s' rule: trace.induct)
-  case (trace_snoc \<tau> s' e s'')
-  then show ?case
-  proof (induction e)
-    case (WCommit x1 x2 x3 x4 x5 x6)
-    then show ?case
-      apply (cases "i = length \<tau>", simp add: tps_trans_defs)
-      by (simp add: length_append_singleton not_less_less_Suc_eq nth_append)
-  qed (simp_all, (smt ev.distinct less_SucE nth_append nth_append_length)+)
-qed simp
-
-lemma WCommit_cts_causal_dep_gt_past:
-  assumes
-    \<open>tps: s \<midarrow>\<langle>\<tau>\<rangle>\<rightarrow> s'\<close>
-    \<open>reach tps s\<close>
-    \<open>k < length \<tau>\<close>
-    \<open>\<tau> ! j = WCommit cl kv_map cts sn u'' clk mmap\<close>
-    \<open>\<tau> ! k = WCommit cl' kv_map' cts' sn' u''' clk' mmap'\<close>
-    \<open>EVI \<tau> j < EVI \<tau> k\<close>
-  shows \<open>(cts, Suc cl) < (cts', Suc cl')\<close>
-  using assms
-proof (induction \<tau> s' rule: trace.induct)
-  case (trace_snoc \<tau> s' e s'')
-  then show ?case
-  proof (induction e)
-    case (WCommit x1 x2 x3 x4 x5 x6)
-    then show ?case apply (simp add: less_prod_def) using WCommit_clk_Suc_cts
-    by (smt (verit) add_less_imp_less_left assms causal_dep_implies_clk_order causal_dep_ind_lt
-        ev_clk.simps(5) ev_i.sel(2) less_ev_i_def less_trans_Suc nth_append plus_1_eq_Suc)
-  qed (simp_all, (smt (verit) Suc_less_SucD causal_dep_ind_lt causal_dep_nth_append ev.distinct
-          ev_i.sel(2) less_ev_i_def less_trans_Suc not_less_less_Suc_eq nth_append nth_append_length')+)
-qed simp
 
 lemma inverted_pair_not_causal_dep:
   assumes
@@ -369,112 +83,162 @@ proof -
   then show ?thesis by force
 qed
 
+
+subsection \<open>measure function lemmas\<close>
+
+lemma i_Suci1:
+  assumes
+    \<open>adj_inv_pair f (l @ e2 # e1 # l') j k\<close>
+    \<open>j \<le> i \<and> Suc i \<le> k\<close>
+    \<open>length l = i\<close>
+    \<open>(i, Suc i) \<noteq> (j, k)\<close>
+  shows "(i, Suc i) \<notin> inverted_pairs f (l @ e2 # e1 # l')"
+  using assms
+  apply (simp add: adj_inv_eq_all_none)
+  apply (simp add: inverted_pairs_def)
+  by (metis Suc_le_lessD le_antisym linorder_le_less_linear option.distinct(1))
+
+lemma i_Suci2:
+  assumes
+    \<open>adj_inv_pair f (l @ e2 # e1 # l') j k\<close>
+    \<open>j \<le> i \<and> Suc i \<le> k\<close>
+    \<open>length l = i\<close>
+  shows "(i, Suc i) \<notin> inverted_pairs f (l @ e1 # e2 # l')"
+  using assms
+  apply (simp add: adj_inv_eq_all_none)
+  apply (simp add: inverted_pairs_def)
+  by (metis Suc_le_lessD leD le_imp_less_Suc le_neq_implies_less nth_append_Suc_length
+      nth_append_length option.discI option.inject order_less_imp_le)
+
+lemma gt_i:
+  assumes
+    \<open>adj_inv_pair f (l @ e2 # e1 # l') j k\<close>
+    \<open>length l = i\<close>
+  shows "\<forall>a > Suc i. (i, a) \<in> inverted_pairs f (l @ e2 # e1 # l') \<longleftrightarrow>
+                 (Suc i, a) \<in> inverted_pairs f (l @ e1 # e2 # l')"
+  using assms
+  apply (auto simp add: inverted_pairs_def)
+  by (metis nth_larger_Suc_length)+
+
+lemma gt_Suci:
+  assumes
+    \<open>adj_inv_pair f (l @ e2 # e1 # l') j k\<close>
+    \<open>length l = i\<close>
+  shows "\<forall>a > Suc i. (Suc i, a) \<in> inverted_pairs f (l @ e2 # e1 # l') \<longleftrightarrow>
+                 (i, a) \<in> inverted_pairs f (l @ e1 # e2 # l')"
+  using assms
+  apply (auto simp add: inverted_pairs_def)
+  by (metis nth_larger_Suc_length)+
+
+lemma lt_i:
+  assumes
+    \<open>adj_inv_pair f (l @ e2 # e1 # l') j k\<close>
+    \<open>length l = i\<close>
+  shows "\<forall>a < i. (a, i) \<in> inverted_pairs f (l @ e2 # e1 # l') \<longleftrightarrow>
+             (a, Suc i) \<in> inverted_pairs f (l @ e1 # e2 # l')"
+  using assms
+  apply (auto simp add: inverted_pairs_def)
+  by (metis nth_append)+
+
+lemma lt_Suci:
+  assumes
+    \<open>adj_inv_pair f (l @ e2 # e1 # l') j k\<close>
+    \<open>length l = i\<close>
+  shows "\<forall>a < i. (a, Suc i) \<in> inverted_pairs f (l @ e2 # e1 # l') \<longleftrightarrow>
+             (a, i) \<in> inverted_pairs f (l @ e1 # e2 # l')"
+  using assms
+  apply (auto simp add: inverted_pairs_def)
+  by (metis nth_append)+
+
+lemma other:
+  assumes
+    \<open>adj_inv_pair f (l @ e2 # e1 # l') j k\<close>
+    \<open>length l = i\<close>
+  shows "\<forall>a b. (a < i \<or> a > Suc i) \<and> (b < i \<or> b > Suc i) \<longrightarrow>
+      (a, b) \<in> inverted_pairs f (l @ e2 # e1 # l') \<longleftrightarrow>
+      (a, b) \<in> inverted_pairs f (l @ e1 # e2 # l')"
+  using assms
+  apply (auto simp add: inverted_pairs_def)
+  by (intro exI, auto simp add: nth_append)
+
 abbreviation swap_i_Suci where
   "swap_i_Suci a i \<equiv> if a = i then Suc i else (if a = Suc i then i else a)"
 
-lemma swap_preserve_reduce_card:
+abbreviation pair_after_swap where
+  "pair_after_swap i \<equiv> (\<lambda>(a, b). (swap_i_Suci a i, swap_i_Suci b i))"
+
+lemma inj_on_pair_after_swap:
+  "inj_on (pair_after_swap i) (inverted_pairs f (l @ e1 # e2 # l'))"
+  apply (auto simp add: inj_on_def)
+  by metis+
+
+lemma pair_after_swap_sound:
+  assumes
+    \<open>adj_inv_pair f (l @ e2 # e1 # l') j k\<close>
+    \<open>j \<le> i \<and> Suc i \<le> k\<close>
+    \<open>length l = i\<close>
+    \<open>(i, Suc i) \<noteq> (j, k)\<close>
+  shows "(pair_after_swap i) ` inverted_pairs f (l @ e1 # e2 # l') =
+         inverted_pairs f (l @ e2 # e1 # l')"
+  apply (auto simp add: image_def)
+  apply (auto dest: inverted_pairs_i_lt_j)
+  apply (metis assms(1,3) gt_i inverted_pairs_i_lt_j)
+  apply (metis assms(1-3) i_Suci2)
+  apply (metis assms(1,3) Suc_lessI gt_Suci inverted_pairs_i_lt_j)
+  apply (metis assms(1,3) inverted_pairs_i_lt_j le_less_Suc_eq linorder_le_less_linear lt_i)
+  apply (metis assms(1,3) inverted_pairs_i_lt_j lt_Suci)
+  subgoal for a b using assms
+    apply (cases "a = i")
+    subgoal apply (cases "b = Suc i")
+      apply metis
+      by (smt (verit) Suc_lessI case_prod_conv gt_i inverted_pairs_i_lt_j leD le_refl)
+    subgoal apply (cases "a = Suc i")
+      apply (smt (verit) gt_Suci inverted_pairs_i_lt_j old.prod.case verit_comp_simplify1(1))
+      apply (cases "b = i"; cases "b = Suc i")
+      apply metis
+      apply (smt (verit) case_prod_conv inverted_pairs_i_lt_j less_le_not_le lt_i)
+      apply (smt (verit) Suc_lessI case_prod_conv inverted_pairs_i_lt_j less_Suc_eq_le
+          less_or_eq_imp_le lt_Suci nat.inject not_less_eq)
+      by (smt (verit, del_insts) Suc_lessI case_prod_conv linorder_neqE_nat other)
+    done
+  subgoal for a b using assms
+    apply (cases "a = i")
+    subgoal apply (cases "b = Suc i")
+      apply (metis (no_types, lifting) i_Suci1)
+      by (smt (verit, del_insts) Suc_lessI case_prod_conv gt_i inverted_pairs_i_lt_j leD le_refl)
+    subgoal apply (cases "a = Suc i")
+      apply (smt (verit, del_insts) gt_Suci inverted_pairs_i_lt_j old.prod.case verit_comp_simplify1(1))
+      apply (cases "b = i"; cases "b = Suc i")
+      apply (metis n_not_Suc_n)
+      apply (smt (verit, del_insts) case_prod_conv inverted_pairs_i_lt_j less_le_not_le lt_i)
+      apply (smt (verit, del_insts) Suc_lessI case_prod_conv inverted_pairs_i_lt_j less_Suc_eq_le
+          less_or_eq_imp_le lt_Suci nat.inject not_less_eq)
+      by (smt (verit, del_insts) Suc_lessI case_prod_conv linorder_neqE_nat other)
+    done
+  done
+
+lemma swap_preserves_card:
   assumes
     \<open>adj_inv_pair f (l @ e2 # e1 # l') j k\<close>
     \<open>j \<le> i \<and> Suc i \<le> k\<close>
     \<open>k < length (l @ e2 # e1 # l')\<close>
     \<open>length l = i\<close>
-  shows "if (i, Suc i) = (j, k)
-    then card (inverted_pairs f (l @ e2 # e1 # l')) = Suc (card (inverted_pairs f (l @ e1 # e2 # l')))
-    else card (inverted_pairs f (l @ e2 # e1 # l')) = card (inverted_pairs f (l @ e1 # e2 # l'))"
+    \<open>(i, Suc i) \<noteq> (j, k)\<close>
+  shows "card (inverted_pairs f (l @ e1 # e2 # l')) = card (inverted_pairs f (l @ e2 # e1 # l'))"
+  using assms
+  apply (intro bij_betw_same_card[of "pair_after_swap i"])
+  by (simp add: bij_betw_def pair_after_swap_sound inj_on_pair_after_swap)
+
+lemma swap_reduces_card:
+  assumes
+    \<open>adj_inv_pair f (l @ e2 # e1 # l') j k\<close>
+    \<open>length l = i\<close>
+    \<open>(i, Suc i) = (j, k)\<close>
+  shows "card (inverted_pairs f (l @ e2 # e1 # l')) = Suc (card (inverted_pairs f (l @ e1 # e2 # l')))"
 proof -
-  have i_Suci1: "(i, Suc i) \<noteq> (j, k) \<Longrightarrow> (i, Suc i) \<notin> inverted_pairs f (l @ e2 # e1 # l')" using assms
-    apply (simp add: adj_inv_eq_all_none)
-    apply (simp add: inverted_pairs_def)
-    by (metis Suc_le_lessD le_antisym linorder_le_less_linear option.distinct(1))
-  have i_Suci2: "(i, Suc i) \<notin> inverted_pairs f (l @ e1 # e2 # l')" using assms
-    apply (simp add: adj_inv_eq_all_none)
-    apply (simp add: inverted_pairs_def)
-    by (metis Suc_le_lessD leD le_imp_less_Suc le_neq_implies_less nth_append_Suc_length
-        nth_append_length option.discI option.inject order_less_imp_le)
-  have gt_i:
-    "\<forall>a > Suc i. (i, a) \<in> inverted_pairs f (l @ e2 # e1 # l') \<longleftrightarrow>
-                 (Suc i, a) \<in> inverted_pairs f (l @ e1 # e2 # l')" using assms
-    apply (auto simp add: inverted_pairs_def)
-    by (metis nth_larger_Suc_length)+
-  have gt_Suci:
-    "\<forall>a > Suc i. (Suc i, a) \<in> inverted_pairs f (l @ e2 # e1 # l') \<longleftrightarrow>
-                 (i, a) \<in> inverted_pairs f (l @ e1 # e2 # l')" using assms
-    apply (auto simp add: inverted_pairs_def)
-    by (metis nth_larger_Suc_length)+
-  have lt_i:
-    "\<forall>a < i. (a, i) \<in> inverted_pairs f (l @ e2 # e1 # l') \<longleftrightarrow>
-             (a, Suc i) \<in> inverted_pairs f (l @ e1 # e2 # l')" using assms
-    apply (auto simp add: inverted_pairs_def)
-    by (metis nth_append)+
-  have lt_Suci:
-    "\<forall>a < i. (a, Suc i) \<in> inverted_pairs f (l @ e2 # e1 # l') \<longleftrightarrow>
-             (a, i) \<in> inverted_pairs f (l @ e1 # e2 # l')" using assms
-    apply (auto simp add: inverted_pairs_def)
-    by (metis nth_append)+
-  have other:
-    "\<forall>a b. (a < i \<or> a > Suc i) \<and> (b < i \<or> b > Suc i) \<longrightarrow>
-      (a, b) \<in> inverted_pairs f (l @ e2 # e1 # l') \<longleftrightarrow>
-      (a, b) \<in> inverted_pairs f (l @ e1 # e2 # l')" using assms
-    apply (auto simp add: inverted_pairs_def)
-    by (intro exI, auto simp add: nth_append)
-  have inj: "inj_on (\<lambda>(a, b). (swap_i_Suci a i, swap_i_Suci b i)) (inverted_pairs f (l @ e1 # e2 # l'))"
-    apply (auto simp add: inj_on_def)
-    by metis+
-  have "(i, Suc i) \<noteq> (j, k) \<Longrightarrow>
-  (\<lambda>x. case x of (a, b) \<Rightarrow> (swap_i_Suci a i, swap_i_Suci b i)) ` inverted_pairs f (l @ e1 # e2 # l') =
-         inverted_pairs f (l @ e2 # e1 # l')"
-    apply (auto simp add: image_def; (auto dest: inverted_pairs_i_lt_j)?)
-    apply (metis gt_i inverted_pairs_i_lt_j)
-    apply (metis i_Suci2)
-    apply (metis Suc_lessI gt_Suci inverted_pairs_i_lt_j)
-    apply (metis inverted_pairs_i_lt_j le_less_Suc_eq linorder_le_less_linear lt_i)
-    apply (metis inverted_pairs_i_lt_j lt_Suci)
-    apply (metis Suc_lessI linorder_neqE_nat other)
-    apply (metis gt_i inverted_pairs_i_lt_j)
-    apply (metis i_Suci2)
-    apply (metis Suc_lessI gt_Suci inverted_pairs_i_lt_j)
-    apply (metis inverted_pairs_i_lt_j le_less_Suc_eq linorder_le_less_linear lt_i)
-    apply (metis inverted_pairs_i_lt_j lt_Suci)
-    apply (metis Suc_lessI nat_neq_iff other)
-    subgoal for a b apply (cases "a = i")
-      subgoal apply (cases "b = Suc i")
-        apply (metis i_Suci1 old.prod.inject)
-        by (smt (verit) Suc_lessI case_prod_conv gt_i inverted_pairs_i_lt_j leD le_refl)
-      subgoal apply (cases "a = Suc i")
-        apply (smt (verit) gt_Suci inverted_pairs_i_lt_j old.prod.case verit_comp_simplify1(1))
-        apply (cases "b = i"; cases "b = Suc i")
-        apply (metis n_not_Suc_n)
-        apply (smt (verit) case_prod_conv inverted_pairs_i_lt_j less_le_not_le lt_i)
-        apply (smt (verit) Suc_lessI case_prod_conv inverted_pairs_i_lt_j less_Suc_eq_le
-            less_or_eq_imp_le lt_Suci nat.inject not_less_eq)
-        by (smt (verit) Suc_lessI case_prod_conv linorder_neqE_nat other)
-      done
-    subgoal for a b apply (cases "a = i")
-      subgoal apply (cases "b = Suc i")
-        apply (metis i_Suci1 old.prod.inject)
-        by (smt (verit) Suc_lessI case_prod_conv gt_i inverted_pairs_i_lt_j leD le_refl)
-      subgoal apply (cases "a = Suc i")
-        apply (smt (verit) gt_Suci inverted_pairs_i_lt_j old.prod.case verit_comp_simplify1(1))
-        apply (cases "b = i"; cases "b = Suc i")
-        apply (metis n_not_Suc_n)
-        apply (smt (verit) case_prod_conv inverted_pairs_i_lt_j less_le_not_le lt_i)
-        apply (smt (verit) Suc_lessI case_prod_conv inverted_pairs_i_lt_j less_Suc_eq_le
-            less_or_eq_imp_le lt_Suci nat.inject not_less_eq)
-        by (smt (verit) Suc_lessI case_prod_conv linorder_neqE_nat other)
-      done
-    done
-  then have card_eq: "(i, Suc i) \<noteq> (j, k) \<Longrightarrow>
-    card (inverted_pairs f (l @ e1 # e2 # l')) = card (inverted_pairs f (l @ e2 # e1 # l'))" using assms
-    apply (intro bij_betw_same_card[of "\<lambda>(a, b). (swap_i_Suci a i, swap_i_Suci b i)"
-        "inverted_pairs f (l @ e1 # e2 # l')" "inverted_pairs f (l @ e2 # e1 # l')"])
-    apply (simp add: bij_betw_def)
-    by (metis inj)
-  have "j = i \<and> Suc i = k \<Longrightarrow> (j, k) \<notin> inverted_pairs f (l @ e1 # e2 # l')"
-    using i_Suci2 by auto
-  then have "j = i \<and> Suc i = k \<Longrightarrow>
-    card (inverted_pairs f (l @ e2 # e1 # l')) = Suc (card (inverted_pairs f (l @ e1 # e2 # l')))" sorry
-  then show ?thesis using card_eq
-    by (metis old.prod.inject)
+  have "(j, k) \<notin> inverted_pairs f (l @ e1 # e2 # l')"
+    using i_Suci2 by (metis Pair_inject assms nat_le_linear)
+  then show ?thesis sorry
 qed
 
 lemma "(ARG_MIN f x. P x) = y \<Longrightarrow> {x. P x} \<noteq> {} \<Longrightarrow> finite {x. P x} \<Longrightarrow> f y = Min (f ` {x. P x})"
@@ -523,16 +287,19 @@ lemma swap_decreases_measure:
   shows \<open>(Exec_frag s0 (efl @ (s, e1, w) # (w, e2, s') # efl') sf, ef) \<in> measure_R\<close>
   using assms
   apply (auto simp add: measure_R_def cons_form_to_index trace_of_decomposed_frag)
-  apply (smt (verit) assms(4) exec_frag.sel(2) length_map lessI swap_preserve_reduce_card
+  subgoal \<comment> \<open>card inverted_pairs\<close>
+    by (smt (verit) assms(4) exec_frag.sel(2) length_map lessI swap_preserves_card
+      swap_reduces_card trace_of_decomposed_frag trace_of_efrag_length)
+  subgoal \<comment> \<open>card lmp_left_movers\<close>
+    apply (cases "(i, Suc i) = (j, k)")
+    subgoal by (smt (verit) assms(4) exec_frag.sel(2) length_map lessI swap_reduces_card
       trace_of_decomposed_frag trace_of_efrag_length)
-  apply (cases "(i, Suc i) = (j, k)")
-  apply (smt (verit) assms(4) exec_frag.sel(2) length_map lessI swap_preserve_reduce_card
-      trace_of_decomposed_frag trace_of_efrag_length)
-
-  
+    subgoal sorry.
+  subgoal \<comment> \<open>dist left_most Lm in lmp from left\<close>
   using trace_of_decomposed_frag [of s0 efl s e2 m e1 s' efl' sf]
   apply (auto simp add: lmp_Lm_dist_left_def trace_of_decomposed_frag split:)
   sorry
+  done
 
 lemma reducible_exec_frag:
   assumes
@@ -578,7 +345,11 @@ proof -
     subgoal using Min_in by blast
     done
   then obtain i where i_: "left_most_Lm (trace_of_efrag ef) i j k" by blast
-  have lc: "left_commute tps (trace_of_efrag ef ! Suc i) (trace_of_efrag ef ! i)" sorry
+  then have "\<not>EVI (trace_of_efrag ef) i < EVI (trace_of_efrag ef) (Suc i)"
+    apply (auto simp add: mover_type_def)
+    by (metis movt.distinct(1) order_less_imp_le order_less_le_trans order_refl)
+  then have lc: "left_commute tps (trace_of_efrag ef ! Suc i) (trace_of_efrag ef ! i)"
+    using indep_evs_commute by auto
   then have reach_si: "reach tps (states_of_efrag ef ! i)"
     by (meson Suc_le_lessD assms(1-2) i_(1) kLen order_less_trans valid_exec_reachable_states)
   then obtain w where
